add completeness

FormalCbgraphs/Graph.lean
@@ -6,22 +6,29 @@ structure Graph where
 
 namespace Graph
 
+variable {G : Graph} {v : G.V}
+
 structure E (G : Graph) where
   u : G.V
   v : G.V
   isEdge : u ∈ G.neighbors v
 
-/-- `Connected Roots Edges v` means a node `v` is connected to a node in `Nodes` via `Edges`. -/
-inductive Connected {G : Graph} (Roots : Set G.V) (Edges : Set G.E) : G.V → Prop where
+/-- `Connected Roots Edges v` means a node `v` is connected to a node in `Roots` via `Edges`. -/
+inductive Connected (Roots : Set G.V) (Edges : Set G.E) : G.V → Prop where
 | base (v : G.V) : v ∈ Roots → Connected Roots Edges v
 | step (e : G.E) : Connected Roots Edges e.u → e ∈ Edges → Connected Roots Edges e.v
 
-/-- `ConnectedWithFailure Roots Edges v k` means a node `v` is connected to a node in `Nodes` via
+/-- `ConnectedWithFailure Roots Edges v k` means a node `v` is connected to a node in `Roots` via
 `Edges` when excluding at most `k` edges arbitrarily. -/
-def ConnectedWithFailure {G : Graph} (Roots : Set G.V) (Edges : Set G.E) (v : G.V) (k : ℕ) :=
+def ConnectedWithFailure (Roots : Set G.V) (Edges : Set G.E) (v : G.V) (k : ℕ) :=
   ∀ (F : Finset G.E), F.card ≤ k → Connected Roots (Edges \ F) v
 
-theorem connectedWithFailure_zero_iff : ConnectedWithFailure Roots Edges v 0 ↔ Connected Roots Edges v := by
+theorem connectedWithFailure_zero_iff {Roots Edges} :
+    ConnectedWithFailure Roots Edges v 0 ↔ Connected Roots Edges v := by
   simp [ConnectedWithFailure]
+
+inductive Path : G.V → Type where
+| nil {u} : Path u
+| cons {u v} : Path u → u ∈ G.neighbors v → Path v
 
 end Graph
